src/PMap.v
@@ -1,0 +1,164 @@
+(** Data Structures
+ ** This file contains efficiently computable implementations of data
+ ** structures aimed at being used in reflective simplification procedures.
+ ** 
+ ** We can't use coq's modular implementations because we have to store
+ ** terms and values that depend on contexts which we can not pre-compute.
+ **)
+Require Import List.
+Require Import Env.
+
+Section FSet.
+  Variable T : Type.
+
+  Definition set := list T.
+
+  Definition set_empty : set := nil.
+End FSet.
+
+Section FMap.
+  Variable K : Type.
+  Variable V : K -> Type.
+
+  Variable Kcmp : forall (a b : K), dcomp a b.
+
+  Inductive dmap : Type :=
+  | DM_Empty : dmap
+  | DM_Branch : forall k, V k -> dmap -> dmap -> dmap.
+
+  Definition dmap_empty : dmap := DM_Empty.
+  
+  Definition dmap_is_empty (d : dmap) : bool :=
+    match d with
+      | DM_Empty => true
+      | _ => false
+    end.
+
+  Variable k : K.
+
+  Fixpoint dmap_lookup (m : dmap): option (V k) :=
+    match m with
+      | DM_Empty => None
+      | DM_Branch k' v' l r =>
+        match Kcmp k' k with
+          | Gt => dmap_lookup l 
+          | Lt => dmap_lookup r
+          | Eq pf => 
+            (** TODO: I don't think this is going to be computable **)
+            match pf in _ = k return option (V k) with
+              | refl_equal => Some v'
+            end
+        end
+    end.
+
+  Fixpoint dmap_insert (v : V k) (m : dmap) : dmap :=
+    match m with
+      | DM_Empty => DM_Branch k v m m 
+      | DM_Branch k' v' l r =>
+        match Kcmp k' k with
+          | Gt => DM_Branch k' v' l (dmap_insert v r)
+          | _ => DM_Branch k' v' (dmap_insert v l) r
+        end
+    end.
+
+  Fixpoint insert_right (l r : dmap) : dmap :=
+    match l with 
+      | DM_Empty => r 
+      | DM_Branch k v ll rr =>
+        DM_Branch k v ll (insert_right rr r)
+    end.
+    
+
+  Fixpoint dmap_remove (m : dmap) : option (V k * dmap) :=
+    match m with
+      | DM_Empty => None
+      | DM_Branch k' v' l r =>
+        match Kcmp k' k with
+          | Gt => match dmap_remove r with
+                    | None => None
+                    | Some (res,m) => Some (res, DM_Branch k' v' l m)
+                  end
+          | Lt => match dmap_remove r with
+                    | None => None
+                    | Some (res,m) => Some (res, DM_Branch k' v' m r)
+                  end
+          | Eq pf =>
+            (** TODO: I don't think this is going to be computable **)
+            Some (match pf in _ = t return V t with
+                    | refl_equal => v' 
+                  end, 
+            match l, r with
+              | DM_Empty , _ => r 
+              | _ , DM_Empty => l
+              | _ , _ => insert_right l r
+            end) 
+        end
+    end.
+
+  Variable T : Type.
+  Variable f : T -> forall k, V k -> T.
+  Fixpoint dmap_fold (a : T) (m : dmap) : T :=
+    match m with
+      | DM_Empty => a
+      | DM_Branch k v l r =>
+        dmap_fold (dmap_fold (f a k v) l) r
+    end.
+  
+End FMap.
+
+Implicit Arguments dmap_empty [ K V ].
+Implicit Arguments dmap_fold [ K V T ].
+Implicit Arguments dmap_remove [ K V ].
+Implicit Arguments dmap_insert [ K V ].
+
+
+(*
+    Parameter map : Type -> Type -> Type.
+
+    Parameter dmap_empty : forall K V, @dmap K V.
+    Parameter dmap_fold : forall {A} {K} {V} (f : A -> forall k, V k -> A) (a : A) (m : @dmap K V), A.
+    Parameter dmap_insert : forall {K} {V} k, V k -> @dmap K V -> dmap V.
+    Parameter dmap_join : forall {K} {V}, @dmap K V -> dmap V -> dmap V.
+    Parameter dmap_remove : forall {K} {V} k, @dmap K V -> option (V k * dmap V).
+    Parameter dmap_is_empty : forall K V (m : @dmap K V), {m = dmap_empty V} + {m <> dmap_empty V}.
+    Parameter map_empty : forall K V, map K V.
+    Parameter map_fold : forall {A} {K} {V} (f : A -> K -> V -> A) (a : A) (m : map K V), A.
+    Parameter map_insert : forall {K} {V}, K -> V -> @map K V -> map K V.
+    Parameter map_join : forall {K} {V}, map K V -> @map K V -> map K V.
+    Parameter map_remove : forall {K} {V}, K -> map K V -> option (V * map K V).    
+
+    Parameter dmap_fold_empty : forall A K V f (a : A), dmap_fold f a (@dmap_empty K V) = a.
+    Parameter map_fold_empty : forall A K V f (a : A), map_fold f a (@map_empty K V) = a.
+*)
+
+
+(*
+Section MMap.
+  Variable K : Type.
+  Variable V : K -> Type.
+  
+  Definition mmap := list {x : K & set (V x)}.
+
+  Variable Keq_dec : forall (a b : K), {a = b} + {a <> b}.
+
+(*
+  Fixpoint lookup (m : mmap) (k : K) : set (V k) :=
+    match m with
+      | nil => set_empty (V k)
+      | existT a b :: r => todo _
+        match Keq_dec k a in { _ } + { _ } return set (V k) with
+          | left _ => b
+          | right _ => todo _
+        end
+    end.
+
+  Fixpoint insert (m : mmap) (k : K) (v : V) : mmap :=
+    match m with
+      | nil => (k, v :: nil) :: nil
+      | (a,b) :: r => 
+        if Keq_dec a k then (a, v :: b) :: r else (a, b) :: insert r k v
+    end.
+*)
+
+End MMap.
+*)
